Unabbreviate cls and lit.

clause.lean
@@ -1,25 +1,25 @@
 import init.meta.tactic utils
 open expr list tactic monad decidable
 
-structure cls :=
+structure clause :=
 (num_quants : ℕ)
 (num_lits : ℕ)
 (has_fin : bool)
 (prf : expr)
 (type : expr)
 
-namespace cls
+namespace clause
 
-private meta def tactic_format (c : cls) : tactic format := do
+private meta def tactic_format (c : clause) : tactic format := do
 prf_fmt : format ← pp (prf c),
 type_fmt ← pp (type c),
 fin_fmt ← return $ to_fmt (if has_fin c then ", has final" else ""),
 return $ prf_fmt ++ to_fmt " : " ++ type_fmt ++ to_fmt " (" ++
   to_fmt (num_quants c) ++ to_fmt " quants, " ++ to_fmt (num_lits c) ++ to_fmt " lits" ++ fin_fmt ++ to_fmt ")"
 
-meta instance : has_to_tactic_format cls := ⟨tactic_format⟩
+meta instance : has_to_tactic_format clause := ⟨tactic_format⟩
 
-def num_binders (c : cls) : ℕ :=
+def num_binders (c : clause) : ℕ :=
 if has_fin c then num_quants c + num_lits c - 1
 else num_quants c + num_lits c
 
@@ -31,39 +31,39 @@ private meta def parse_clause_type : expr → ℕ × ℕ × bool
   end
 | e := if expr.is_false e then (0, 0, ff) else (0, 1, tt)
 
-meta def of_proof_and_type (prf type : expr) : cls :=
+meta def of_proof_and_type (prf type : expr) : clause :=
 match parse_clause_type type with
 (qs, ls, fin) := mk qs ls fin prf type
 end
 
-meta def of_proof (prf : expr) : tactic cls := do
+meta def of_proof (prf : expr) : tactic clause := do
 type ← infer_type prf,
 return $ of_proof_and_type prf type
 
-meta def validate (c : cls) : tactic unit := do
+meta def validate (c : clause) : tactic unit := do
 type' ← infer_type c↣prf,
 unify c↣type type' <|> (do pp_ty ← pp c↣type, pp_ty' ← pp type',
                            fail (to_fmt "wrong type: " ++ pp_ty ++ " =!= " ++ pp_ty'))
 
-meta def inst (c : cls) (e : expr) : cls :=
+meta def inst (c : clause) (e : expr) : clause :=
 (if num_quants c > 0
   then mk (num_quants c - 1) (num_lits c)
   else mk 0 (num_lits c - 1)) (has_fin c)
 (app (prf c) e) (instantiate_var (binding_body (type c)) e)
 
-meta def instn (c : cls) (es : list expr) : cls :=
+meta def instn (c : clause) (es : list expr) : clause :=
 foldr (λe c', inst c' e) c es
 
-meta def open_const (c : cls) : tactic (cls × expr) := do
+meta def open_const (c : clause) : tactic (clause × expr) := do
 n ← mk_fresh_name,
 b ← return $ local_const n (binding_name (type c)) (binding_info (type c)) (binding_domain (type c)),
 return (inst c b, b)
 
-meta def open_meta (c : cls) : tactic (cls × expr) := do
+meta def open_meta (c : clause) : tactic (clause × expr) := do
 b ← mk_meta_var (binding_domain (type c)),
 return (inst c b, b)
 
-meta def close_const (c : cls) (e : expr) : cls :=
+meta def close_const (c : clause) (e : expr) : clause :=
 match e with
 | local_const uniq pp info t :=
     let abst_type' := abstract_local (type c) (local_uniq_name e) in
@@ -76,69 +76,69 @@ match e with
 | _ := mk 0 0 tt (mk_var 0) (mk_var 0)
 end
 
-meta def open_constn : cls → ℕ → tactic (cls × list expr)
+meta def open_constn : clause → ℕ → tactic (clause × list expr)
 | c 0 := return (c, nil)
 | c (n+1) := do
   (c', b) ← open_const c,
   (c'', bs) ← open_constn c' n,
   return (c'', b::bs)
 
-meta def open_metan : cls → ℕ → tactic (cls × list expr)
+meta def open_metan : clause → ℕ → tactic (clause × list expr)
 | c 0 := return (c, nil)
 | c (n+1) := do
   (c', b) ← open_meta c,
   (c'', bs) ← open_metan c' n,
   return (c'', b::bs)
 
-meta def close_constn : cls → list expr → cls
+meta def close_constn : clause → list expr → clause
 | c [] := c
 | c (b::bs') := close_const (close_constn c bs') b
 
-meta def inst_mvars (c : cls) : tactic cls := do
+meta def inst_mvars (c : clause) : tactic clause := do
 prf' ← instantiate_mvars (prf c),
 type' ← instantiate_mvars (type c),
 return { c with prf := prf', type := type' }
 
-inductive lit
-| left : expr → lit
-| right : expr → lit
-| final : expr → lit
+inductive literal
+| left : expr → literal
+| right : expr → literal
+| final : expr → literal
 
-namespace lit
+namespace literal
 
-meta instance : decidable_eq lit := by mk_dec_eq_instance
+meta instance : decidable_eq literal := by mk_dec_eq_instance
 
-def formula : lit → expr
+def formula : literal → expr
 | (left f) := f
 | (right f) := f
 | (final f) := f
 
-def is_neg : lit → bool
+def is_neg : literal → bool
 | (left _) := tt
 | (right _) := ff
 | (final _) := ff
 
-def is_pos (l : lit) : bool := bnot l↣is_neg
+def is_pos (l : literal) : bool := bnot l↣is_neg
 
-def is_final : lit → bool
+def is_final : literal → bool
 | (final _) := tt
 | _ := ff
 
-meta def to_formula (l : lit) : tactic expr :=
+meta def to_formula (l : literal) : tactic expr :=
 if is_neg l then mk_mapp ``not [some (formula l)]
 else return (formula l)
 
-meta def type_str : lit → string
-| (lit.left _) := "left"
-| (lit.right _) := "right"
-| (lit.final _) := "final"
+meta def type_str : literal → string
+| (literal.left _) := "left"
+| (literal.right _) := "right"
+| (literal.final _) := "final"
 
-meta instance : has_to_tactic_format lit :=
+meta instance : has_to_tactic_format literal :=
 ⟨λl, do
 pp_f ← pp l↣formula,
 return $ to_fmt l↣type_str ++ " (" ++ pp_f ++ ")"⟩
 
-end lit
+end literal
 
 private meta def get_binding_body : expr → ℕ → expr
 | e 0 := e
@@ -147,24 +147,24 @@ private meta def get_binding_body : expr → ℕ → expr
 meta def get_binder (e : expr) (i : nat) :=
 binding_domain (get_binding_body e i)
 
-meta def get_lit (c : cls) (i : nat) : lit :=
-if has_fin c ∧ num_lits c = i + 1 then lit.final (get_binding_body (type c) (num_quants c + i))
+meta def get_lit (c : clause) (i : nat) : literal :=
+if has_fin c ∧ num_lits c = i + 1 then literal.final (get_binding_body (type c) (num_quants c + i))
 else let bind := get_binder (type c) (num_quants c + i) in
 match is_not bind with
-| some formula := lit.right formula
-| none := lit.left bind
+| some formula := literal.right formula
+| none := literal.left bind
 end
 
-meta def lits_where (c : cls) (p : lit → bool) : list nat :=
+meta def lits_where (c : clause) (p : literal → bool) : list nat :=
 list.filter (λl, p (get_lit c l)) (range (num_lits c))
 
-meta def get_lits (c : cls) : list lit :=
+meta def get_lits (c : clause) : list literal :=
 list.map (get_lit c) (range c↣num_lits)
 
-meta def is_maximal (gt : expr → expr → bool) (c : cls) (i : nat) : bool :=
+meta def is_maximal (gt : expr → expr → bool) (c : clause) (i : nat) : bool :=
 list.empty (filter (λj, gt (get_lit c j)↣formula (get_lit c i)↣formula) (range c↣num_lits))
 
-meta def normalize (c : cls) : tactic cls := do
+meta def normalize (c : clause) : tactic clause := do
 opened  ← open_constn c (num_binders c),
 lconsts_in_types ← return $ contained_lconsts_list (list.map local_type opened.2),
 quants' ← return $ filter (λlc, rb_map.contains lconsts_in_types (local_uniq_name lc)) opened.2,
@@ -172,15 +172,15 @@ lits' ← return $ filter (λlc, ¬rb_map.contains lconsts_in_types (local_uniq_
 return $ close_constn opened.1 (quants' ++ lits')
 
 lemma fin_to_pos_helper {p} (Hp : p) : (p → false) → false := take Hnp, Hnp Hp
-meta def fin_to_pos (c : cls) : tactic cls :=
+meta def fin_to_pos (c : clause) : tactic clause :=
 if ¬has_fin c then return c else do
 op ← open_constn c c↣num_binders,
 prf' ← mk_mapp ``fin_to_pos_helper [some (type op.1), some (prf op.1)],
 type' ← return $ imp (imp op↣1↣type false_) false_,
 return $ close_constn (mk 0 1 ff prf' type') op.2
 
-private meta def focus' (c : cls) (i : nat) : tactic cls := do
-guard $ lit.is_pos (get_lit c i),
+private meta def focus' (c : clause) (i : nat) : tactic clause := do
+guard $ literal.is_pos (get_lit c i),
 qf ← c↣open_constn c↣num_quants,
 op ← qf↣1↣open_constn c↣num_lits,
 hyp_i ← (op↣2↣nth i)↣to_monad,
@@ -188,7 +188,7 @@ prf' ← mk_mapp ``classical.by_contradiction [none, some (lambdas [hyp_i] op↣
 type' ← return (qf↣1↣get_lit i)↣formula,
 return $ close_constn ⟨0, 1, tt, prf', type'⟩ (qf↣2 ++ op↣2↣remove i)
 
-meta def focus (c : cls) (i : nat) : tactic cls :=
+meta def focus (c : clause) (i : nat) : tactic clause :=
 if has_fin c ∧ i+1 = num_lits c then
   return c
 else if has_fin c then
@@ -196,20 +196,20 @@ else if has_fin c then
 else
   focus' c i
 
-meta def whnf_head_lit (c : cls) : tactic cls := do
-atom' ← whnf (lit.formula $ get_lit c 0),
+meta def whnf_head_lit (c : clause) : tactic clause := do
+atom' ← whnf (literal.formula $ get_lit c 0),
 return $ if c↣has_fin ∧ c↣num_lits = 1 ∧ c↣num_quants = 0 then
   { c with type := atom' }
-else if lit.is_neg (get_lit c 0) then
+else if literal.is_neg (get_lit c 0) then
   { c with type := imp atom' (binding_body c↣type) }
 else
   { c with type := imp (app (const ``not []) atom') c↣type↣binding_body }
 
-end cls
+end clause
 
-meta def unify_lit (l1 l2 : cls.lit) : tactic unit :=
-if cls.lit.is_pos l1 = cls.lit.is_pos l2 then
-  unify_core transparency.none (cls.lit.formula l1) (cls.lit.formula l2)
+meta def unify_lit (l1 l2 : clause.literal) : tactic unit :=
+if clause.literal.is_pos l1 = clause.literal.is_pos l2 then
+  unify_core transparency.none (clause.literal.formula l1) (clause.literal.formula l2)
 else
   fail "cannot unify literals"
 
@@ -235,11 +235,11 @@ match list.filter (λm, ¬has_meta_var (get_meta_type m)) metas with
 | _ := failed
 end
 
-namespace cls
+namespace clause
 
-meta def meta_closure (metas : list expr) (qf : cls) : tactic cls := do
+meta def meta_closure (metas : list expr) (qf : clause) : tactic clause := do
 bs ← sort_and_constify_metas metas,
-qf' ← cls.inst_mvars qf,
-cls.inst_mvars $ cls.close_constn qf' bs
+qf' ← clause.inst_mvars qf,
+clause.inst_mvars $ clause.close_constn qf' bs
 
-end cls
+end clause
