equality.lean
@@ -1,9 +1,9 @@
 import clause prover_state utils
 open tactic monad expr list
 
-meta def try_unify_eq_l (c : cls) (i : nat) : tactic cls := do
-guard $ cls.lit.is_neg (cls.get_lit c i),
-qf ← cls.open_metan c c↣num_quants,
+meta def try_unify_eq_l (c : clause) (i : nat) : tactic clause := do
+guard $ clause.literal.is_neg (clause.get_lit c i),
+qf ← clause.open_metan c c↣num_quants,
 match is_eq (qf↣1↣get_lit i)↣formula with
 | none := failed
 | some (lhs, rhs) := do
@@ -11,19 +11,19 @@ unify lhs rhs,
 ty ← infer_type lhs,
 univ ← infer_univ ty,
 refl ← return $ app_of_list (const ``eq.refl [univ]) [ty, lhs],
-opened ← cls.open_constn qf↣1 i,
-cls.meta_closure qf↣2 $ cls.close_constn (opened↣1↣inst refl) opened↣2
+opened ← clause.open_constn qf↣1 i,
+clause.meta_closure qf↣2 $ clause.close_constn (opened↣1↣inst refl) opened↣2
 end
 
 meta def unify_eq_inf : inference := take given, sequence' $ do
 i ← given↣selected,
 [(do u ← resolution_prover_of_tactic $ try_unify_eq_l given↣c i, add_inferred u [given]) <|> return ()]
 
-meta def has_refl_r (c : cls) : bool :=
+meta def has_refl_r (c : clause) : bool :=
 list.bor $ do
-lit ← c↣get_lits,
-guard lit↣is_pos,
-match is_eq lit↣formula with
+literal ← c↣get_lits,
+guard literal↣is_pos,
+match is_eq literal↣formula with
 | some (lhs, rhs) := [decidable.to_bool (lhs = rhs)]
 | none := []
 end
