factoring.lean
@@ -3,26 +3,26 @@ open tactic expr monad
 
 variable gt : expr → expr → bool
 
-meta def inst_lit (c : cls) (i : nat) (e : expr) : tactic cls := do
-opened ← cls.open_constn c i,
-return $ cls.close_constn (cls.inst opened.1 e) opened.2
+meta def inst_lit (c : clause) (i : nat) (e : expr) : tactic clause := do
+opened ← clause.open_constn c i,
+return $ clause.close_constn (clause.inst opened.1 e) opened.2
 
-private meta def try_factor' (c : cls) (i j : nat) : tactic cls := do
-qf ← cls.open_metan c c↣num_quants,
+private meta def try_factor' (c : clause) (i j : nat) : tactic clause := do
+qf ← clause.open_metan c c↣num_quants,
 unify_lit (qf↣1↣get_lit i) (qf↣1↣get_lit j),
-qfi ← cls.inst_mvars qf.1,
-guard $ cls.is_maximal gt qfi i,
-at_j ← cls.open_constn qf.1 j,
+qfi ← clause.inst_mvars qf.1,
+guard $ clause.is_maximal gt qfi i,
+at_j ← clause.open_constn qf.1 j,
 hyp_i ← option.to_monad (list.nth at_j.2 i),
 cs ← sort_and_constify_metas qf.2,
-qf' ← cls.inst_mvars $
-  if cls.has_fin c ∧ j+1 = cls.num_lits c then
-    cls.close_constn (cls.of_proof_and_type (app hyp_i at_j.1↣prf) (const ``false [])) at_j.2
+qf' ← clause.inst_mvars $
+  if clause.has_fin c ∧ j+1 = clause.num_lits c then
+    clause.close_constn (clause.of_proof_and_type (app hyp_i at_j.1↣prf) (const ``false [])) at_j.2
   else
-    cls.close_constn (cls.inst at_j.1 hyp_i) at_j.2,
-return $ cls.close_constn qf' cs
+    clause.close_constn (clause.inst at_j.1 hyp_i) at_j.2,
+return $ clause.close_constn qf' cs
 
-meta def try_factor (c : cls) (i j : nat) : tactic cls :=
+meta def try_factor (c : clause) (i j : nat) : tactic clause :=
 if i > j then try_factor' gt c j i else try_factor' gt c i j
 
 meta def try_infer_factor (c : active_cls) (i j : nat) : resolution_prover unit := do
@@ -37,7 +37,7 @@ take given, do gt ← get_term_order, sequence' $ do
   j ← list.range given↣c↣num_lits,
   return $ try_infer_factor gt given i j <|> return ()
 
-meta def factor_dup_lits' : cls → tactic cls | c :=
+meta def factor_dup_lits' : clause → tactic clause | c :=
 match (do i ← c↣get_lits↣zip_with_index,
           j ← c↣get_lits↣zip_with_index,
           guard $ i↣2 < j↣2,
@@ -47,7 +47,7 @@ match (do i ← c↣get_lits↣zip_with_index,
 | [] := return c
 end
 
-meta def factor_dup_lits (c : cls) : tactic cls := do
+meta def factor_dup_lits (c : clause) : tactic clause := do
 qf ← c↣open_constn c↣num_quants,
 qf' ← factor_dup_lits' qf↣1,
 return $ qf'↣close_constn qf↣2
