misc_preprocessing.lean
@@ -1,16 +1,16 @@
 import clause prover_state
 open expr list monad
 
-meta def is_taut (c : cls) : tactic bool := do
-qf ← cls.open_constn c c↣num_quants,
+meta def is_taut (c : clause) : tactic bool := do
+qf ← clause.open_constn c c↣num_quants,
 return $ list.bor (do
-  l1 ← cls.get_lits qf.1, guard $ cls.lit.is_neg l1,
-  l2 ← cls.get_lits qf.1, guard $ cls.lit.is_pos l2,
-  [decidable.to_bool (cls.lit.formula l1 = cls.lit.formula l2)])
+  l1 ← clause.get_lits qf.1, guard $ clause.literal.is_neg l1,
+  l2 ← clause.get_lits qf.1, guard $ clause.literal.is_pos l2,
+  [decidable.to_bool (clause.literal.formula l1 = clause.literal.formula l2)])
 
 open tactic
 example (i : Type) (p : i → i → Type) (c : i) (h : ∀ (x : i), p x c → p x c) : true := by do
-h ← get_local `h, hcls ← monad.liftM (cls.mk 1 2 tt h) (infer_type h),
+h ← get_local `h, hcls ← monad.liftM (clause.mk 1 2 tt h) (infer_type h),
 taut ← is_taut hcls,
 when (¬taut) failed,
 to_expr `(trivial) >>= apply
@@ -20,11 +20,11 @@ preprocessing_rule $ λnew, resolution_prover_of_tactic (filterM (λc, liftM bno
 
 meta def remove_duplicates_pre : resolution_prover unit :=
 preprocessing_rule $ λnew,
-return (rb_map.values (rb_map.of_list (list.map (λc:cls, (c↣type, c)) new)))
+return (rb_map.values (rb_map.of_list (list.map (λc:clause, (c↣type, c)) new)))
 
 meta def only_pos_to_fin_pre : resolution_prover unit :=
 preprocessing_rule $ take news, flip mapM news $ take new, do
-match list.filter (λl : (cls.lit × ℕ), l↣1↣is_pos) new↣get_lits↣zip_with_index with
+match list.filter (λl : (clause.literal × ℕ), l↣1↣is_pos) new↣get_lits↣zip_with_index with
 | [l] := do univ ← resolution_prover_of_tactic $ infer_univ l↣1↣formula,
             if ¬l↣1↣is_final ∧ univ = level.zero then
               resolution_prover_of_tactic (new↣focus l↣2)
