resolution.lean
@@ -3,22 +3,22 @@ open tactic monad
 
 variable gt : expr → expr → bool
 variables (ac1 ac2 : active_cls)
-variables (c1 c2 : cls)
+variables (c1 c2 : clause)
 variables (i1 i2 : nat)
 
 -- c1 : ... → a
 -- c2 : ... → a → ...
-meta def try_resolve : tactic cls := do
-qf1 ← cls.open_metan c1 c1↣num_quants,
-qf2 ← cls.open_metan c2 c2↣num_quants,
-unify (cls.lit.formula (cls.get_lit qf1.1 i1)) (cls.lit.formula (cls.get_lit qf2.1 i2)),
-qf1i ← cls.inst_mvars qf1.1,
-guard $ cls.is_maximal gt qf1i i1,
-focused_qf1 ← cls.focus qf1.1 i1,
-op1 ← cls.open_constn focused_qf1 focused_qf1↣num_binders,
-op2 ← cls.open_constn qf2.1 i2,
-cls.meta_closure (qf1.2 ++ qf2.2) $
-  cls.close_constn (cls.inst op2.1 op1↣1↣prf) (op1.2 ++ op2.2)
+meta def try_resolve : tactic clause := do
+qf1 ← clause.open_metan c1 c1↣num_quants,
+qf2 ← clause.open_metan c2 c2↣num_quants,
+unify (clause.literal.formula (clause.get_lit qf1.1 i1)) (clause.literal.formula (clause.get_lit qf2.1 i2)),
+qf1i ← clause.inst_mvars qf1.1,
+guard $ clause.is_maximal gt qf1i i1,
+focused_qf1 ← clause.focus qf1.1 i1,
+op1 ← clause.open_constn focused_qf1 focused_qf1↣num_binders,
+op2 ← clause.open_constn qf2.1 i2,
+clause.meta_closure (qf1.2 ++ qf2.2) $
+  clause.close_constn (clause.inst op2.1 op1↣1↣prf) (op1.2 ++ op2.2)
 
 meta def try_add_resolvent : resolution_prover unit := do
 c' ← resolution_prover_of_tactic $ try_resolve gt ac1↣c ac2↣c i1 i2,
@@ -30,19 +30,19 @@ try_add_resolvent gt ac1 ac2 i1 i2 <|> return ()
 meta def resolution_left_inf : inference :=
 take given, do active : rb_map name active_cls ← get_active, sequence' $ do
   given_i ← given↣selected,
-  guard $ cls.lit.is_neg (given↣c↣get_lit given_i),
+  guard $ clause.literal.is_neg (given↣c↣get_lit given_i),
   other ← rb_map.values active,
   other_i ← other↣selected,
-  guard $ cls.lit.is_pos (other↣c↣get_lit other_i),
+  guard $ clause.literal.is_pos (other↣c↣get_lit other_i),
   [maybe_add_resolvent gt other given other_i given_i]
 
 meta def resolution_right_inf : inference :=
 take given, do active : rb_map name active_cls ← get_active, sequence' $ do
   given_i ← given↣selected,
-  guard $ cls.lit.is_pos (given↣c↣get_lit given_i),
+  guard $ clause.literal.is_pos (given↣c↣get_lit given_i),
   other ← rb_map.values active,
   other_i ← other↣selected,
-  guard $ cls.lit.is_neg (other↣c↣get_lit other_i),
+  guard $ clause.literal.is_neg (other↣c↣get_lit other_i),
   [maybe_add_resolvent gt given other given_i other_i]
 
 meta def resolution_inf : inference :=
